\documentclass[a4,draft]{article}
\usepackage{amsmath}
\begin{document}

\section{Forward/backward movement}

\begin{eqnarray}
  f(t) &=& \begin{cases} 
    f_1(t)=\frac{a}{\alpha}t & -\alpha \leq t \le  \alpha\\
    f_2(t - \pi) & \alpha \leq t \le  \pi \\
    f_3(t - \pi) &  \pi \leq t \le  2\pi -\alpha
  \end{cases}\\
  f_2''(t) &=& Jt + C_1\\
  f_2'(t) &=& J\frac{t^2}{2} + C_1t + C_2 \\
  f_2(t) &=& J\frac{t^3}{6} + C_1\frac{t^2}{2} + C_2t + C_3 \\
  f_2(\alpha - \pi) &=& a \\
  f_2(0) &=& 0 \\
  f_2''(\alpha - \pi) &=& 0 \\
  f_2'(\alpha - \pi) &=& \frac{a}{\alpha}
\end{eqnarray}

\begin{eqnarray}
  \beta &=& \alpha - \pi \\
  C_1 &=& -J\beta \\
  C_2 &=& \frac{a}{\alpha} - J\frac{\beta^2}{2} +J\beta^2 = \frac{a}{\alpha} + J\frac{\beta^2}{2}\\
  C_3 &=& 0 \\
  a &=&J\frac{\beta^3}{6} -J\beta\frac{\beta^2}{2} + \left(\frac{a}{\alpha} + J\frac{\beta^2}{2}\right)\beta \\
  a &=& J\beta^3\left(\frac{1}{6} - \frac{1}{2} + \frac{1}{2}\right) + \frac{a\beta}{\alpha} \\
  J &=& \frac{6\pi a}{\alpha \beta^3} \\
  f_2(t) &=& J\frac{t^3}{6} -J\beta\frac{t^2}{2} + \left(\frac{a}{\alpha} + J\frac{\beta^2}{2}\right) t \\
  f_2(t) &=& \frac{a}{\alpha} \left( \frac{6\pi}{\beta^3}\left(\frac{1}{6}t^3 -\frac{\beta}{2}t^2 + \frac{\beta^2}{2} t \right) +  t \right) \\
  f_2'(t) &=& J\frac{t^2}{2} -J\beta t + \left(\frac{a}{\alpha} + J\frac{\beta^2}{2}\right) \\
  f_2''(t) &=& J t - J\beta
\end{eqnarray}
\begin{eqnarray}
  f_3(t) &=& -f_2(-t)
\end{eqnarray}

\section{Up/down movement}
\begin{eqnarray}
  f(t) &=& \begin{cases} 
    0 & -\alpha \leq t \le  \alpha\\
    f_4(t - \pi) & \alpha \leq t \le \pi \\
    f_5(t - \pi) & \pi \leq t \le  2\pi -\alpha
  \end{cases}\\
  \beta &=& \alpha - \pi \\
  f_4''(t) &=& Jt + A \\
  f_4'(t) &=& J\frac{t^2}{2} + At + V \\
  f_4(t) &=& J\frac{t^3}{6} + A\frac{t^2}{2} + Vt + S \\
  f_4(\beta) &=& 0 \\
  f_4(0) &=& h\\
  f_4'(\beta) &=& 0 \\
  f_4'(0) &=& 0
\end{eqnarray}

\begin{eqnarray}
  S &=& h \\
  V &=& 0 \\
  0 &=& J\frac{\beta^2}{2} + A\beta \\
  0 &=& J\frac{\beta^3}{6} + A\frac{\beta^2}{2} + h\\
  0 &=& J\frac{\beta^3}{4} - J\frac{\beta^3}{6} - h\\
  0 &=& J\beta^3\left(\frac{1}{4} - \frac{1}{6}\right) - h\\
  0 &=& J\beta^3\left(\frac{1}{12}\right) - h\\
  J &=& \frac{12h}{\beta^3} \\
  A&=&-\frac{12h}{\beta^3}\frac{\beta}{2}=-\frac{6h}{\beta^2}\\
  f_4(t) &=& \frac{2h}{\beta^3}t^3 - \frac{3h}{\beta^2}t^2 + h = \frac{2ht^2}{\beta^2}(2t - 3\beta) + h
\end{eqnarray}
\end{document}
